theory/MasterLR.dfy
@@ -1,4 +1,3 @@
-
 include "./math/ExpReal.dfy"
 include "./math/FloorCeil.dfy"
 include "./math/LemBoundsNat.dfy"
